proof/algo/ln_inf_extra.v
@@ -1,0 +1,63 @@
+Require Import Coq.Program.Equality.
+
+Require Import algo.ott.
+Require Export algo.notations.
+
+
+
+Lemma la_type_subst_open_comm : forall x t1 A t2,
+  lc_la_type t1 -> 
+  x `notin` fx_la_type t2 -> 
+  ([t1 /ᵃ x] A) ^^ᵃ t2 = [t1 /ᵃ x] A ^^ᵃ t2.
+Proof.
+  intros.
+  rewrite subst_la_type_open_la_type_wrt_la_type.
+  rewrite (subst_la_type_fresh_eq t2).
+  all: easy.
+Qed.
+
+
+
+
+Lemma fx_la_type_open_la_type_notin_rec : forall x e2,
+  x `notin` fx_la_type e2 -> 
+  forall e1 n, 
+    x `notin` fx_la_type e1 ->
+    x `notin` fx_la_type (open_la_type_wrt_la_type_rec n e2 e1).
+Proof.
+  intros until e1.
+  induction e1; simpl; intros; auto.
+  - destruct (lt_eq_lt_dec n n0). destruct s.
+    all: auto.
+Qed.
+
+Lemma fx_la_type_open_la_type_notin : forall x e1 e2, 
+  x `notin` fx_la_type e1 -> 
+  x `notin` fx_la_type e2 -> 
+  x `notin` fx_la_type (e1 ^^ᵃ e2).
+Proof.
+  intros.
+  eauto using fx_la_type_open_la_type_notin_rec.
+Qed.
+
+
+Lemma fex_la_type_open_la_type_notin_rec : forall x e2,
+  x `notin` fex_la_type e2 -> 
+  forall e1 n, 
+    x `notin` fex_la_type e1 ->
+    x `notin` fex_la_type (open_la_type_wrt_la_type_rec n e2 e1).
+Proof.
+  intros until e1.
+  induction e1; simpl; intros; auto.
+  - destruct (lt_eq_lt_dec n n0). destruct s.
+    all: auto.
+Qed.
+
+Lemma fex_la_type_open_la_type_notin : forall x e1 e2, 
+  x `notin` fex_la_type e1 -> 
+  x `notin` fex_la_type e2 -> 
+  x `notin` fex_la_type (e1 ^^ᵃ e2).
+Proof.
+  intros.
+  eauto using fex_la_type_open_la_type_notin_rec.
+Qed.
