proof/decl/ln_inf_extra.v
@@ -2,12 +2,25 @@ Require Import decl.ott.
 Require Export decl.notations.
 
 
+
+Lemma ld_type_subst_open_comm : forall x t1 A t2,
+  lc_ld_type t1 -> 
+  x `notin` fv_ld_type t2 -> 
+  ([t1 /ᵈ x] A) ^^ᵈ t2 = [t1 /ᵈ x] A ^^ᵈ t2.
+Proof.
+  intros.
+  rewrite subst_ld_type_open_ld_type_wrt_ld_type.
+  rewrite (subst_ld_type_fresh_eq t2).
+  all: easy.
+Qed.
+
+
 Lemma ld_type_open_r_close_l : forall t1 t2 x
   , x `notin` fv_ld_type t2
-  -> t1 = open_ld_type_wrt_ld_type t2 `x -> close_ld_type_wrt_ld_type x t1 = t2.
+  -> t1 = open_ld_type_wrt_ld_type t2 `ᵈ x -> close_ld_type_wrt_ld_type x t1 = t2.
 Proof.
   intros * Fr H.
-  assert (close_ld_type_wrt_ld_type x t1 = close_ld_type_wrt_ld_type x (open_ld_type_wrt_ld_type t2 `x)) by now rewrite H.
+  assert (close_ld_type_wrt_ld_type x t1 = close_ld_type_wrt_ld_type x (open_ld_type_wrt_ld_type t2 `ᵈ x)) by now rewrite H.
   now rewrite close_ld_type_wrt_ld_type_open_ld_type_wrt_ld_type in H0.
 Qed.
 
