proof/decl/properties.v
@@ -29,7 +29,7 @@ Tactic Notation "pick" "fresh" ident(x) "and" "apply" constr(H) "for" "weakening
   apply_fresh_base_fixed H gather_for_weakening x.
 
 Lemma subst_same_eq : forall A x,
-  A = [`x /ᵈ x] A.
+  A = [`ᵈ x /ᵈ x] A.
 Proof.
   intros.
   induction A; auto.
@@ -41,7 +41,7 @@ Qed.
 
 Lemma open_subst_eq : forall A x t, 
   x `notin` fv_ld_type A -> lc_ld_type t  ->
-    A ^^ᵈ t = [t /ᵈ x] A ^^ᵈ `x.
+    A ^^ᵈ t = [t /ᵈ x] A ^^ᵈ (`ᵈ x).
 Proof.
   intros.  
   rewrite subst_ld_type_open_ld_type_wrt_ld_type. simpl.
@@ -69,7 +69,7 @@ Qed.
 
 
 Lemma ld_sub_refl :
-  forall G A, ld_wf_type G A -> ld_sub G A A.
+  forall G A, ld_wf_type G A -> G ⊢ A <: A.
 Proof.
   intros.
   induction H.
@@ -77,7 +77,7 @@ Proof.
   - constructor; auto.
   - constructor; auto.
   - eapply ld_sub_forallr with (L:=L `union` (ld_ctx_dom G)). intros. 
-    inst_cofinites_with x. eapply ld_sub_foralll with (t := `x); auto.
+    inst_cofinites_with x. eapply ld_sub_foralll with (t := (`ᵈ x)); auto.
     constructor.
     + eapply ld_sub_wf_ctx; eauto.
     + simpl. auto. 
@@ -85,7 +85,7 @@ Qed.
 
 
 Lemma ld_sub_mono_symm : 
-  forall G t1 t2, ld_mono_type t1 -> ld_mono_type t2 -> ld_sub G t1 t2 -> ld_sub G t2 t1.
+  forall G t1 t2, ld_mono_type t1 -> ld_mono_type t2 -> G ⊢ t1 <: t2 -> G ⊢ t2 <: t1.
 Proof.
   intros.
   dependent induction H1; auto.
@@ -239,8 +239,8 @@ Qed.
 Ltac rewrite_subst_open_var :=
   repeat
     match goal with 
-      | _ : _ |-  context [ ([?e /ᵈ ?x] ?A) ^^ᵈ ` ?x' ] => 
-        replace (` x') with ([e /ᵈ x] `x') by (apply subst_ld_type_fresh_eq; auto)
+      | _ : _ |-  context [ ([?e /ᵈ ?x] ?A) ^^ᵈ (`ᵈ ?x') ] => 
+        replace (`ᵈ x') with ([e /ᵈ x] (`ᵈ x')) by (apply subst_ld_type_fresh_eq; auto)
     end; repeat rewrite <- subst_ld_type_open_ld_type_wrt_ld_type by auto.
 
 
@@ -278,7 +278,7 @@ Proof.
   - simpl. eapply ld_sub_forallr with (L:=L `union` singleton x).
     intros. inst_cofinites_with x0.
     rewrite_subst_open_var.
-    replace  (([t /ᵈ x] B) ^^ᵈ ([t /ᵈ x] ` x0)) with ( [t /ᵈ x] B ^^ᵈ ` x0).
+    replace  (([t /ᵈ x] B) ^^ᵈ ([t /ᵈ x] `ᵈ x0)) with ( [t /ᵈ x] B ^^ᵈ `ᵈ x0).
     + replace (G1,, G2, x0 ) with (G1,, (G2, x0)) by auto. apply H0; auto.
     + rewrite subst_ld_type_open_ld_type_wrt_ld_type. reflexivity. simpl.
       replace (G1,, G2, x0 ) with (G1,, (G2, x0)) by auto. now apply ld_mono_is_ld_lc.
@@ -407,7 +407,7 @@ Qed.
 Theorem sized_var_substitution : forall G1 G2 x x' A B n,
   G1 , x  ,, G2 ⊢ A <: B | n ->
   ⊢ G1, x' ,, G2 ->
-  G1 , x' ,, G2 ⊢ [`x' /ᵈ x] A <: [`x' /ᵈ x] B | n.
+  G1 , x' ,, G2 ⊢ [(`ᵈ x') /ᵈ x] A <: [(`ᵈ x') /ᵈ x] B | n.
 Proof with auto with trans.
   intros. dependent induction H; simpl; auto...
   - simpl. destruct (x0 == x). 
@@ -418,9 +418,9 @@ Proof with auto with trans.
       * auto.
       * eapply ld_in_context_other in H0; eauto.
         replace (G1,x',,G2) with (G1,,(ld_ctx_nil, x'),,G2) by auto. apply ld_in_context_weakenning. auto.
-  - simpl. eapply sls_foralll with (t:=[`x' /ᵈ x] t). 
+  - simpl. eapply sls_foralll with (t:=[`ᵈ x' /ᵈ x] t). 
     + destruct (x==x'); subst.
-      * replace ([` x' /ᵈ x'] t) with t; auto.
+      * replace ([`ᵈ x' /ᵈ x'] t) with t; auto.
         now apply subst_same_eq.
       * apply ld_wf_mtype_equiv_ld_wf_type_and_mono in H. destruct H.
         apply ld_wf_mtype_subst.
@@ -436,13 +436,13 @@ Proof with auto with trans.
                simpl. rewrite <- IHG2. auto.
         -- constructor. replace (G1, x') with (G1,x',,ld_ctx_nil) by auto. eapply ld_wf_ctx_weakening; eauto.
            constructor. 
-    + replace (([`x' /ᵈ x] A) ^^ᵈ ([`x' /ᵈ x] t)) with ([`x' /ᵈ x] A ^^ᵈ t).
+    + replace (([`ᵈ x' /ᵈ x] A) ^^ᵈ ([`ᵈ x' /ᵈ x] t)) with ([`ᵈ x' /ᵈ x] A ^^ᵈ t).
       * apply IHsized_ld_sub; auto.
       * rewrite subst_ld_type_open_ld_type_wrt_ld_type; auto. 
   - simpl. eapply sls_forallr with (L:=L `union` singleton x `union` ld_ctx_dom ( G1, x',, G2)).
     intros. inst_cofinites_with x0.
     rewrite_subst_open_var.
-    replace  (([`x' /ᵈ x] B) ^^ᵈ ([`x' /ᵈ x] ` x0)) with ( [`x' /ᵈ x] B ^^ᵈ ` x0).
+    replace  (([(`ᵈ x') /ᵈ x] B) ^^ᵈ ([(`ᵈ x') /ᵈ x] `ᵈ x0)) with ( [(`ᵈ x') /ᵈ x] B ^^ᵈ `ᵈ x0).
     + replace (G1, x',, G2, x0 ) with (G1,x',, (G2, x0)) by auto. apply H0; auto.
       simpl. constructor; auto. 
     + rewrite subst_ld_type_open_ld_type_wrt_ld_type. reflexivity. simpl.
@@ -471,8 +471,8 @@ Proof with eauto with trans.
   + inst_cofinites_by (L `union` fv_ld_type A `union` fv_ld_type B). destruct H0 as [n].
     exists (S n). eapply sls_forallr with (L:=L `union` (ld_ctx_dom G)). intros.
     replace (G, x0) with (G, x0,,ld_ctx_nil) by auto.
-    replace A with ([`x0 /ᵈ x] A).
-    replace (B ^^ᵈ `x0) with ([`x0 /ᵈ x] B ^^ᵈ `x).
+    replace A with ([`ᵈ x0 /ᵈ x] A).
+    replace (B ^^ᵈ `ᵈ x0) with ([`ᵈ x0 /ᵈ x] B ^^ᵈ `ᵈ x).
     eapply sized_var_substitution; eauto.
     * simpl. auto.
       apply ld_sub_wf_ctx in H. dependent destruction H. auto.
@@ -520,7 +520,7 @@ Proof with eauto with trans.
           eapply IHt_order with (B:=B ^^ᵈ t) (n1:=n1) (n2:=n0); eauto. simpl in H; eauto.
           rewrite (open_mono_order B t); eauto...
           replace G with (G ,, ld_ctx_nil) by auto.
-          replace (B ^^ᵈ t) with ([t /ᵈ x] B ^^ᵈ `x).
+          replace (B ^^ᵈ t) with ([t /ᵈ x] B ^^ᵈ `ᵈ x).
           replace A with ([t /ᵈ x] A).
           -- auto. 
           -- rewrite subst_ld_type_fresh_eq; auto.
@@ -534,8 +534,8 @@ Proof with eauto with trans.
           assert (⊢ G, x0). { constructor. dependent destruction H5;  auto. auto. }
           replace (G, x, x0) with (G ,, (ld_ctx_nil,  x) ,, (ld_ctx_nil, x0)) by auto.
           eapply sized_ld_sub_weakening; simpl.
-          replace A with ([`x0 /ᵈ x] A).
-          replace (B ^^ᵈ `x0) with ([`x0 /ᵈ x] B ^^ᵈ `x).
+          replace A with ([`ᵈ x0 /ᵈ x] A).
+          replace (B ^^ᵈ `ᵈ x0) with ([`ᵈ x0 /ᵈ x] B ^^ᵈ `ᵈ x).
           replace (G, x0) with (G, x0,, ld_ctx_nil) by auto.
           apply sized_var_substitution; auto.
           -- apply eq_sym. eauto... 
