proof/ln_utils.v
@@ -4,6 +4,11 @@ Require Export Metalib.Metatheory.
 Require Import decl.notations.
 Require Import algo.notations.
 
+
+Notation "x ∉ L" := (x `notin` L)
+  (at level 65, no associativity).
+
+
 Ltac inst_cofinite_impl H x :=
   match type of H with
   | forall x, x `notin` ?L -> _ =>
@@ -12,6 +17,7 @@ Ltac inst_cofinite_impl H x :=
       specialize (H x Fr); clear Fr
   end
 .
+
 
 Ltac inst_cofinites_with x :=
   repeat
@@ -40,7 +46,7 @@ Ltac rewrite_la_subst_open_var :=
   repeat
     match goal with 
       | _ : _ |-  context [ ([?e /ᵃ ?x] ?A) ^ᵃ ?x' ] => 
-        replace (`′ x') with ([ e /ᵃ x ] `′ x') by (apply subst_la_type_fresh_eq; auto)
+        replace (`ᵃ x') with ([ e /ᵃ x ] (`ᵃ x')) by (apply subst_la_type_fresh_eq; auto)
     end; repeat rewrite <- subst_la_type_open_la_type_wrt_la_type by auto.
 
 
@@ -48,5 +54,5 @@ Ltac rewrite_ld_subst_open_var :=
   repeat
     match goal with 
       | _ : _ |-  context [ ([?e /ᵈ ?x] ?A) ^ᵈ ?x' ] => 
-        replace (` x') with ([ e /ᵈ x ] ` x') by (apply subst_ld_type_fresh_eq; auto)
+        replace (`ᵈ x') with ([ e /ᵈ x ] `ᵈ x') by (apply subst_ld_type_fresh_eq; auto)
     end; repeat rewrite <- subst_ld_type_open_ld_type_wrt_ld_type by auto.
